Busybeaver.lean
@@ -1,3 +1,11 @@
 -- This module serves as the root of the `Busybeaver` library.
 -- Import modules here that should be built as part of the library.
 import Busybeaver.Basic
+import Busybeaver.Reachability
+
+open TM
+
+variable {l s: ℕ}
+
+def filterWith (S: Finset (Machine l s)) (filter: (M: Machine l s) → HaltM M Unit): Finset (Machine l s) :=
+  S.filter $ λ m ↦ ¬(filter m |>.decided)
