Main.lean
@@ -1,8 +1,22 @@
+import Busybeaver
 import Busybeaver.Basic
 import Busybeaver.Deciders.LooperDec
 import Busybeaver.Deciders.BoundExplore
+import Busybeaver.Deciders.NoHaltState
 
-def main (args: List String): IO UInt32 := do
-  for M in (Finset.univ (α:=TM.Machine 2 2)) do
-    IO.println s!"{repr M}"
+def main (_args: List String): IO UInt32 := do
+  IO.println "Hewo"
   return 0
+
+open TM
+
+abbrev TM22 := Machine 1 1
+
+def all22 := Finset.univ (α:=TM22)
+#eval all22.card
+
+def withHalt := filterWith all22 noHaltDec
+#eval withHalt.card
+
+def long22 := filterWith withHalt (looperDec 100)
+#eval long22.card
